extracted ~ low

src/specs/permutationQuotientContribution.ec
@@ -1,40 +1,94 @@
 pragma Goals:printall.
 
-require import AllCore Int IntDiv Constants Field.
+require import AllCore Int IntDiv.
+require import Constants Field Verifier UInt256 YulPrimops PurePrimops VerifierConsts.
 
 module PermutationQuotientContribution = {
-  var a4, a5, b, g : Fr
-  var zp_z0, l0_z : Fr
-  var s0_z, s1_z, s2_z, s3_z : Fr
-  var a_z, b_z, c_z : Fr
- 
-  proc high() : Fr = {
-    var s0BGa, s1BGb, s2BGc, s3G : Fr;
 
-    s0BGa <- s0_z * b + g + a_z;
-    s1BGb <- s1_z * b + g + b_z;
-    s2BGc <- s2_z * b + g + c_z;
-    s3G   <- s3_z + g;
+  proc low(): uint256 = {
+    var usr_res, a4, zperm_zo, usr_gamma, usr_beta, usr_factorMultiplier, sigma0_z, a_z, sigma1_z, b_z, sigma2_z, c_z, sigma3_z, _22, l0AtZ, a5, _26;
+    a4 <@ Primops.mload(STATE_POWER_OF_ALPHA_4_SLOT);
+    zperm_zo <@ Primops.mload(PROOF_COPY_PERMUTATION_GRAND_PRODUCT_OPENING_AT_Z_OMEGA_SLOT);
+    usr_res <- (PurePrimops.mulmod a4 zperm_zo (W256.of_int R));
     
-    return (-(a4 * zp_z0 * s0BGa * s1BGb * s2BGc * s3G)) - (a5 * l0_z);
+    usr_gamma <@ Primops.mload(STATE_GAMMA_SLOT);
+    usr_beta <@ Primops.mload(STATE_BETA_SLOT);
+    
+    sigma0_z <@ Primops.mload(PROOF_COPY_PERMUTATION_POLYS_0_OPENING_AT_Z_SLOT);
+    usr_factorMultiplier <- (PurePrimops.mulmod sigma0_z usr_beta (W256.of_int R));
+    usr_factorMultiplier <- (PurePrimops.addmod usr_factorMultiplier usr_gamma (W256.of_int R));
+    a_z <@ Primops.mload(PROOF_STATE_POLYS_0_OPENING_AT_Z_SLOT);
+    usr_factorMultiplier <- (PurePrimops.addmod usr_factorMultiplier a_z (W256.of_int R));
+    usr_res <- (PurePrimops.mulmod usr_res usr_factorMultiplier (W256.of_int R));
+    
+    sigma1_z <@ Primops.mload(PROOF_COPY_PERMUTATION_POLYS_1_OPENING_AT_Z_SLOT);
+    usr_factorMultiplier <- (PurePrimops.mulmod sigma1_z usr_beta (W256.of_int R));
+    usr_factorMultiplier <- (PurePrimops.addmod usr_factorMultiplier usr_gamma (W256.of_int R));
+    b_z <@ Primops.mload(PROOF_STATE_POLYS_1_OPENING_AT_Z_SLOT);
+    usr_factorMultiplier <- (PurePrimops.addmod usr_factorMultiplier b_z (W256.of_int R));
+    usr_res <- (PurePrimops.mulmod usr_res usr_factorMultiplier (W256.of_int R));
+    
+    sigma2_z <@ Primops.mload(PROOF_COPY_PERMUTATION_POLYS_2_OPENING_AT_Z_SLOT);
+    usr_factorMultiplier <- (PurePrimops.mulmod sigma2_z usr_beta (W256.of_int R));
+    usr_factorMultiplier <- (PurePrimops.addmod usr_factorMultiplier usr_gamma (W256.of_int R));
+    c_z <@ Primops.mload(PROOF_STATE_POLYS_2_OPENING_AT_Z_SLOT);
+    usr_factorMultiplier <- (PurePrimops.addmod usr_factorMultiplier c_z (W256.of_int R));
+    usr_res <- (PurePrimops.mulmod usr_res usr_factorMultiplier (W256.of_int R));
+    
+    sigma3_z <@ Primops.mload(PROOF_STATE_POLYS_3_OPENING_AT_Z_SLOT);
+    _22 <- (PurePrimops.addmod sigma3_z usr_gamma (W256.of_int R));
+    usr_res <- (PurePrimops.mulmod usr_res _22 (W256.of_int R));
+    usr_res <- ((W256.of_int R) - usr_res);
+    
+    l0AtZ <@ Primops.mload(STATE_L_0_AT_Z_SLOT);
+    a5 <@ Primops.mload(STATE_POWER_OF_ALPHA_5_SLOT);
+    l0AtZ <- (PurePrimops.mulmod l0AtZ a5 (W256.of_int R));
+    _26 <- ((W256.of_int R) - l0AtZ);
+    usr_res <- (PurePrimops.addmod usr_res _26 (W256.of_int R));
+
+    return usr_res;
   }
+
+  (* var a4, a5, b, g : Fr *)
+  (* var zp_z0, l0_z : Fr *)
+  (* var s0_z, s1_z, s2_z, s3_z : Fr *)
+  (* var a_z, b_z, c_z : Fr *)
  
-  var _a4, _a5, _b, _g : int
-  var _zp_z0, _l0_z : int
-  var _s0_z, _s1_z, _s2_z, _s3_z : int
-  var _a_z, _b_z, _c_z : int
+  (* proc high() : Fr = { *)
+  (*   var s0BGa, s1BGb, s2BGc, s3G : Fr; *)
+
+  (*   s0BGa <- s0_z * b + g + a_z; *)
+  (*   s1BGb <- s1_z * b + g + b_z; *)
+  (*   s2BGc <- s2_z * b + g + c_z; *)
+  (*   s3G   <- s3_z + g; *)
+    
+  (*   return (-(a4 * zp_z0 * s0BGa * s1BGb * s2BGc * s3G)) - (a5 * l0_z); *)
+  (* } *)
+ 
+  (* var _a4, _a5, _b, _g : int *)
+  (* var _zp_z0, _l0_z : int *)
+  (* var _s0_z, _s1_z, _s2_z, _s3_z : int *)
+  (* var _a_z, _b_z, _c_z : int *)
   
-  proc mid() : int = {
-    var s0BGa, s1BGb, s2BGc, s3G : int;
+  (* proc mid() : int = { *)
+  (*   var s0BGa, s1BGb, s2BGc, s3G : int; *)
 
-    s0BGa <- (_s0_z * _b + _g + _a_z)%%R;
-    s1BGb <- (_s1_z * _b + _g + _b_z)%%R;
-    s2BGc <- (_s2_z * _b + _g + _c_z)%%R;
-    s3G   <- (_s3_z + _g)%%R;
+  (*   s0BGa <- (_s0_z * _b + _g + _a_z)%%R; *)
+  (*   s1BGb <- (_s1_z * _b + _g + _b_z)%%R; *)
+  (*   s2BGc <- (_s2_z * _b + _g + _c_z)%%R; *)
+  (*   s3G   <- (_s3_z + _g)%%R; *)
 
-    return ((R - (_a4 * _zp_z0 * s0BGa * s1BGb * s2BGc * s3G)) + (R - (_a5 * _l0_z)))%%R;
-  }  
+  (*   return ((R - (_a4 * _zp_z0 * s0BGa * s1BGb * s2BGc * s3G)) + (R - (_a5 * _l0_z)))%%R; *)
+  (* }   *)
 }.
+
+lemma permutationQuotientContribution_extracted_equiv_low :
+equiv [Verifier.usr_permutationQuotientContribution ~ PermutationQuotientContribution.low :
+      ={arg, glob PermutationQuotientContribution} ==> ={res, glob PermutationQuotientContribution}].
+proof. proc.
+inline *; wp; skip; progress; smt ().
+qed.
+
 
 (* op permutationQuotientContribution_Mspec *)
 (*   (A4 A5 zperm_zO L0_z *)
