src/Field.ec
@@ -1,6 +1,5 @@
 pragma Goals:printall.
 
-<<<<<<< HEAD
 require import AllCore Int IntDiv ZModP StdOrder.
 require import Constants.
 
@@ -36,30 +35,3 @@ op (^) (x : FieldR.F) (k : int) = FieldR.exp x k axiomatized by RexpE.
 (*   rewrite domain_sizeFrE /asint /inFr; have ->: DOMAIN_SIZE %% R = DOMAIN_SIZE by smt. *)
 (*   rewrite Sub.insubdK //; smt. *)
 (* qed. *)
-=======
-require import AllCore Int IntDiv ZModP.
-require import Constants.
-
-clone include ZModField  with 
-  op p <- R 
-  rename "zmod" as "Fr"
-  rename "ZModp" as "Zr"
-  proof prime_p by apply prime_r.
-   
-op (^) (x : Fr) (k : int) = exp x k axiomatized by expE.
-
-op OMEGAFr = inFr OMEGA axiomatized by omegaFrE.
-op DOMAIN_SIZEFr = inFr DOMAIN_SIZE axiomatized by domain_sizeFrE.
-
-lemma omega_eq_omegaFr : asint OMEGAFr = OMEGA.
-proof.
-  rewrite omegaFrE /asint /inFr; have ->: OMEGA %% R = OMEGA by smt.
-  rewrite Sub.insubdK //; smt.
-qed.
-
-lemma domain_eq_domainFr : asint DOMAIN_SIZEFr = DOMAIN_SIZE.
-proof.
-  rewrite domain_sizeFrE /asint /inFr; have ->: DOMAIN_SIZE %% R = DOMAIN_SIZE by smt.
-  rewrite Sub.insubdK //; smt.
-qed.
->>>>>>> 207ac17 (refined specs.)
